Introduced kv_appears_in_kvl and kv_appears_in_tree, and changed everything.

code/InductiveDataTypes.v
@@ -15,27 +15,55 @@ Example test := bptLeaf 2 bool [(1, true), (2, false)].
 
 
 Inductive appears_in_kvl {X:Type} (sk: nat) : list (nat * X) -> Prop :=
-  | aik_here : forall v l, appears_in_kvl sk ((sk, v)::l)
-  | aik_later : forall k v l, appears_in_kvl sk l -> appears_in_kvl sk ((k, v)::l).
+  | aik_here: forall v l,		appears_in_kvl sk ((sk, v)::l)
+  | aik_later: forall k v l,	appears_in_kvl sk l -> appears_in_kvl sk ((k, v)::l).
+
+Inductive kv_appears_in_kvl {X:Type} (sk: nat) (sv: X) : list (nat * X) -> Prop :=
+  | kv_aik_here: forall l,		kv_appears_in_kvl sk sv ((sk, sv)::l)
+  | kv_aik_later: forall k v l,	kv_appears_in_kvl sk sv l -> kv_appears_in_kvl sk sv ((k, v)::l).
+  
+Lemma kv_appears_in_kvl_impl_appears_in_kvl: forall (X: Type) (k: nat) (v: X) (l: list (nat * X)),
+  kv_appears_in_kvl k v l -> appears_in_kvl k l.
+Proof.
+  intros.
+  induction H; constructor; assumption.
+Qed.
   
 Inductive appears_in_tree {X:Type} {b: nat} (sk: nat) : bplustree b X -> Prop :=
-  | ait_leaf          : forall l,       appears_in_kvl sk l -> appears_in_tree sk (bptLeaf b X l)
-  | ait_node_last : forall k1 k2 v1 v2, appears_in_tree sk v2 -> k2 <= sk ->
-                                     appears_in_tree sk (bptNode b X [(k1, v1), (k2, v2)])
-  | ait_node_here  : forall k1 k2 v1 v2 l, 
-                                     appears_in_tree sk v1 -> k1 <= sk /\ sk < k2 ->
-                                     appears_in_tree sk (bptNode b X ((k1, v1)::(k2, v2)::l))
-  | ait_node_later : forall x k1 k2 v1 v2 l, appears_in_tree sk (bptNode b X ((k1, v1)::(k2, v2)::l)) -> k1 <= sk ->
-                                     appears_in_tree sk (bptNode b X (x::(k1, v1)::(k2, v2)::l)).
+  | ait_leaf: forall l,	appears_in_kvl sk l -> appears_in_tree sk (bptLeaf b X l)
+  | ait_node_last: forall k1 k2 v1 v2, 
+		appears_in_tree sk v2 -> k2 <= sk ->
+		appears_in_tree sk (bptNode b X [(k1, v1), (k2, v2)])
+  | ait_node_here: forall k1 k2 v1 v2 l, 
+		appears_in_tree sk v1 -> k1 <= sk /\ sk < k2 ->
+		appears_in_tree sk (bptNode b X ((k1, v1)::(k2, v2)::l))
+  | ait_node_later: forall x k1 k2 v1 v2 l,
+  		appears_in_tree sk (bptNode b X ((k1, v1)::(k2, v2)::l)) -> 
+  		k1 <= sk ->
+		appears_in_tree sk (bptNode b X (x::(k1, v1)::(k2, v2)::l)).
+
+Inductive kv_appears_in_tree {X:Type} {b: nat} (sk: nat) (sv: X) : bplustree b X -> Prop :=
+  | kv_ait_leaf: forall l,	kv_appears_in_kvl sk sv l -> kv_appears_in_tree sk sv (bptLeaf b X l)
+  | kv_ait_node_last: forall k1 k2 v1 v2, 
+		kv_appears_in_tree sk sv v2 -> k2 <= sk ->
+		kv_appears_in_tree sk sv (bptNode b X [(k1, v1), (k2, v2)])
+  | kv_ait_node_here: forall k1 k2 v1 v2 l, 
+		kv_appears_in_tree sk sv v1 -> k1 <= sk /\ sk < k2 ->
+		kv_appears_in_tree sk sv (bptNode b X ((k1, v1)::(k2, v2)::l))
+  | kv_ait_node_later: forall x k1 k2 v1 v2 l,
+  		kv_appears_in_tree sk sv (bptNode b X ((k1, v1)::(k2, v2)::l)) -> 
+  		k1 <= sk ->
+		kv_appears_in_tree sk sv (bptNode b X (x::(k1, v1)::(k2, v2)::l)).
   
   
 Inductive kvl_sorted {X: Type}: list (nat * X) -> Prop :=
-  kvl_sorted_0    : kvl_sorted []
-| kvl_sorted_1    : forall (n: nat) (x: X), 
-                      kvl_sorted [(n, x)]
-| kvl_sorted_cons : forall (n1 n2: nat) (x1 x2: X) (lst: list (nat * X)), 
-                      kvl_sorted ((n2,x2)::lst) -> blt_nat n1 n2 = true
-                       -> kvl_sorted ((n1,x1)::(n2,x2)::lst) .
+    kvl_sorted_0    : kvl_sorted []
+  | kvl_sorted_1    : forall (n: nat) (x: X), 
+		kvl_sorted [(n, x)]
+  | kvl_sorted_cons : forall (n1 n2: nat) (x1 x2: X) (lst: list (nat * X)), 
+		kvl_sorted ((n2,x2)::lst) -> 
+		blt_nat n1 n2 = true ->
+		kvl_sorted ((n1,x1)::(n2,x2)::lst).
                        
 (* Some props for having a prop apply to all elements in a list *)
 Inductive all_values (X : Type) (P : X -> Prop) : list (nat * X) -> Prop :=
