code/AppearsInKVL.v
@@ -26,6 +26,15 @@ Proof.
   exists ((k0, v)::witness). exists witness0. exists witness1. simpl. rewrite cons_remove. apply H2.
 Qed.
 
+Lemma kv_appears_in_kvl_app : forall (X: Type) (k: nat) (v: X) (l: list (nat*X)),
+  kv_appears_in_kvl k v l -> exists l1, exists l2, l = l1++(k,v)::l2.
+Proof.
+  intros X k v l H. induction H. exists []. exists l. reflexivity.
+  inversion IHkv_appears_in_kvl. inversion H0. inversion H1.
+  exists ((k0, v0)::witness). exists witness0. 
+  simpl. reflexivity.
+Qed.
+
 Lemma appears_in_super_set_appears : forall (X: Type) k (x: (nat*X)) (l l': list (nat*X)),
   x :: l' = l -> appears_in_kvl k l' -> appears_in_kvl k l.
 Proof.
@@ -35,7 +44,14 @@ Proof.
   apply IHappears_in_kvl with (x:= (k0, v)). reflexivity.
 Qed.
 
-
+Lemma kv_appears_in_super_set_appears : forall (X: Type) k v (x: (nat*X)) (l l': list (nat*X)),
+  x :: l' = l -> kv_appears_in_kvl k v l' -> kv_appears_in_kvl k v l.
+Proof.
+  intros. generalize dependent l. generalize dependent x. induction H0. intros. 
+  rewrite <- H. destruct x. apply kv_aik_later. apply kv_aik_here.
+  intros. destruct l0. inversion H. inversion H. destruct p. apply kv_aik_later.
+  apply IHkv_appears_in_kvl with (x:= (k0, v0)). reflexivity.
+Qed.
 
 Lemma appears_in_kvl_dist_app : forall (X: Type) (k: nat) (l l1 l2: list (nat*X)),
   l = l1++l2 -> appears_in_kvl k l -> 
@@ -54,6 +70,25 @@ Proof.
         appears_in_kvl k ((k0, v) :: l1) \/ appears_in_kvl k l2). 
         intros. destruct H1. left. apply aik_later. assumption. right. assumption. 
     apply H1. apply IHappears_in_kvl. apply H3.
+Qed.
+
+Lemma kv_appears_in_kvl_dist_app : forall (X: Type) (k: nat) (v: X) (l l1 l2: list (nat*X)),
+  l = l1++l2 -> kv_appears_in_kvl k v l -> 
+  kv_appears_in_kvl k v l1 \/ kv_appears_in_kvl k v l2.
+Proof.
+  intros. generalize dependent l1. induction H0; intros.
+  Case "kv_aik_here".
+    destruct l1. destruct l2; inversion H. destruct p. 
+    inversion H1. right. apply kv_aik_here.
+    destruct p. inversion H. left. apply kv_aik_here.
+  Case "kv_aik_later".
+    destruct l1. simpl in H. right. eapply kv_appears_in_super_set_appears. apply H. assumption.
+    inversion H. 
+      assert(
+        kv_appears_in_kvl k v l1 \/ kv_appears_in_kvl k v l2 ->
+        kv_appears_in_kvl k v ((k0, v0) :: l1) \/ kv_appears_in_kvl k v l2). 
+        intros. destruct H1. left. apply kv_aik_later. assumption. right. assumption. 
+    apply H1. apply IHkv_appears_in_kvl. apply H3.
 Qed.
 
 Theorem appears_kvl_appears_leaf_tree: forall {X: Type} (b: nat) k l,
@@ -76,13 +111,27 @@ Proof.
   apply H2.
 Qed.
 
+Lemma kv_appears_cons : forall (X: Type) (k k1: nat) (v v1: X) (l: list (nat*X)),
+  kv_appears_in_kvl k v ((k1, v1) :: l) -> 
+  k <> k1 -> 
+  kv_appears_in_kvl k v (l).
+Proof.
+  intros.
+  inversion H.
+  subst.
+  apply ex_falso_quodlibet. omega.
+  subst.
+  apply H2.
+Qed.
+
+
 Theorem insert_into_list_appears : forall (X: Type) (l: list (nat * X)) (k: nat) (v: X),
-  appears_in_kvl k (insert_into_list k v l).
+  kv_appears_in_kvl k v (insert_into_list k v l).
 Proof.
   intros.
   induction l.
   Case "l = []".
-    simpl. apply aik_here.
+    simpl. apply kv_aik_here.
   Case "l = a::l".
     destruct a. simpl. 
     remember (ble_nat k n) as klen. 
@@ -90,11 +139,11 @@ Proof.
     SCase "k <= n". remember (beq_nat k n) as keqn. 
       destruct keqn; symmetry in Heqkeqn; [apply beq_nat_true_iff in Heqkeqn | apply beq_nat_false_iff in Heqkeqn].
       SSCase "k = n".
-        apply aik_here.
+        apply kv_aik_here.
       SSCase "k <> n".
-      apply aik_here.
+      apply kv_aik_here.
     SCase "k > n".
-      apply aik_later. apply IHl.
+      apply kv_aik_later. apply IHl.
 Qed.
 
 
