code/InsertSearchWorksProofs.v
@@ -2,6 +2,7 @@ Require Export BPlusTree.
 Require Export SortingProofs.
 Require Export ValidBPlusTree.
 Require Export InsertWorksProofs.
+Require Export InsertPreservesProofs.
 Require Export SearchWorksProofs.
 
 Theorem insert_words: forall {X: Type} {b: nat} (k: nat) (v: X) (t: bplustree b X),
@@ -9,13 +10,13 @@ Theorem insert_words: forall {X: Type} {b: nat} (k: nat) (v: X) (t: bplustree b 
   ~ appears_in_tree k t ->
   search k (insert k v t) = Some (v).
 Proof.
-  intros. remember (insert k v t). symmetry in Heqb0. apply insert_works in Heqb0.
-  Case "Search in tree finds some element".
-    apply appears_search_works in Heqb0. destruct Heqb0. 
-    admit.
-    admit.
-  assumption. assumption.
-Admitted.
+  intros. remember (insert k v t). symmetry in Heqb0.
+  assert (valid_bplustree b X b0).
+    apply insert_preserves_valid_bplustree with (k := k) (v := v) in H.
+    rewrite Heqb0 in H. apply H.
+  apply insert_works in Heqb0; try assumption.
+  apply appears_search_works in Heqb0; assumption. 
+Qed.
 
 Theorem insert_into_list_works : forall (X: Type) (l: list (nat * X)) (k: nat) (v: X),
   kvl_sorted l -> search_leaf k (insert_into_list k v l) = Some v. 
