code/InsertWorksProofs.v
@@ -9,6 +9,7 @@ Require Export ElementAtIndexProofs.
 Require Export SplitCutList.
 Require Export FindSubtreeProofs.
 Require Export InsertProofs.
+Require Export KvAppearsInTree.
   
 Lemma list_of_length_b_implies_element_at_b : forall (X: Type) (b: nat) (kvl: list (nat* X)),
   kvl <> [] -> b < length kvl -> 
@@ -34,7 +35,7 @@ Qed.
 Theorem split_insert_right : forall {X: Type} {b: nat} (leaf left kvl: list (nat * X)) (k kb: nat) (v vb: X),
   b <> 0 -> kvl_sorted leaf -> not (appears_in_kvl k leaf) -> element_at_index (pred b) leaf = Some (kb, vb) -> 
   kb < k -> length leaf = mult b 2 -> 
-  insert_leaf b k v leaf = (left, Some kvl) -> appears_in_kvl k kvl.
+  insert_leaf b k v leaf = (left, Some kvl) -> kv_appears_in_kvl k v kvl.
 Proof.
   intros. 
   
@@ -64,7 +65,7 @@ Proof.
          apply split_list_preserves_lists in Heqsplit.
          assert ((n, x) :: insert_into_list k v leaf = left ++ kvl) by assumption.
          
-         apply appears_in_kvl_dist_app with (k := k) in Heqsplit.
+         apply kv_appears_in_kvl_dist_app with (k := k) (v := v) in Heqsplit.
          inversion Heqsplit. clear Heqsplit. 
          SSSSCase "appears_in_kvl n left".
            (* This case is bogus, needs an inversion *)
@@ -76,7 +77,7 @@ Proof.
            apply element_at_index_pred_b_implies_left_below_S_b with (l1 := left) (l2 := kvl) in H2; try assumption.
            apply key_greater_than_all_keys_does_not_appear_ble with (k:=k) in H2; try assumption.
            (* We've found our inversion - k both appears and does not appear in left *)
-           apply ex_falso_quodlibet. apply H2. assumption.
+           apply ex_falso_quodlibet. apply H2. apply kv_appears_in_kvl_impl_appears_in_kvl in H8. assumption.
            
             
            (* Now we just need to prove all of the assumptions *)            
@@ -94,7 +95,7 @@ Proof.
            reflexivity.
          SSSSCase "appears_in_kvl n kvl".
            assumption.
-         apply aik_later.
+         apply kv_aik_later.
          apply insert_into_list_appears.
          unfold not. intro. apply H1. apply aik_later. assumption.
        SSSCase "n = k".
@@ -131,7 +132,7 @@ Qed.
 Theorem split_insert_left : forall {X: Type} {b: nat} (leaf left kvl: list (nat * X)) (k kb: nat) (v vb: X),
   b <> 0 -> kvl_sorted leaf -> not (appears_in_kvl k leaf) -> element_at_index (pred b) leaf = Some (kb, vb) -> 
   k < kb -> length leaf = mult b 2 ->
-  insert_leaf b k v leaf = (left, Some kvl) -> appears_in_kvl k left.
+  insert_leaf b k v leaf = (left, Some kvl) -> kv_appears_in_kvl k v left.
 Proof.
   intros.
   destruct leaf.
@@ -181,10 +182,10 @@ Proof.
          SSSSCase "left = p::left". 
            destruct p.
            rewrite <- app_comm_cons in Heqsplit. inversion Heqsplit.
-           apply appears_in_kvl_dist_app with (k := k) in H11.
+           apply kv_appears_in_kvl_dist_app with (k := k) (v := v) in H11.
            destruct H11.
            SSSSSCase "appears in left".
-             apply aik_later. apply H8.
+             apply kv_aik_later. apply H8.
            SSSSSCase "appears in right".
              (* This case is bogus *)
              symmetry in H7. apply split_list_left_length in H7. 
@@ -200,7 +201,7 @@ Proof.
              apply element_at_index_b_implies_right_above_b with (l1 := ((n0,x0)::left)) (l2 := kvl) in H2.
              apply key_smaller_than_all_keys_does_not_appear with (k:= k) in H2.
              
-             apply ex_falso_quodlibet. apply H2. assumption.
+             apply ex_falso_quodlibet. apply H2. apply kv_appears_in_kvl_impl_appears_in_kvl in H8. assumption.
              symmetry in Heqsplit. 
              assert (kvl_sorted ((n, x) :: insert_into_list k v leaf)).
                apply insert_preserves_sort_cons.
@@ -245,14 +246,14 @@ Proof.
               omega.
             SSSCase "left = p::left".
               destruct p.
-              rewrite <- app_comm_cons in Heqsplit. inversion Heqsplit. apply aik_here.
+              rewrite <- app_comm_cons in Heqsplit. inversion Heqsplit. apply kv_aik_here.
               omega.
 Qed.
 
 
 Theorem insert_leaf_normal : forall {X: Type} {b: nat} (leaf left: list (nat * X)) (k: nat) (v: X),
   b <> 0 -> kvl_sorted leaf -> not (appears_in_kvl k leaf) -> length leaf < mult b 2 ->
-  insert_leaf b k v leaf = (left, None) -> appears_in_kvl k left.
+  insert_leaf b k v leaf = (left, None) -> kv_appears_in_kvl k v left.
 Proof.
   intros. 
   
@@ -260,7 +261,7 @@ Proof.
   Case "leaf = []".
     intros.
     destruct b. apply ex_falso_quodlibet. apply H. reflexivity.
-    compute in H3. inversion H3. apply aik_here.
+    compute in H3. inversion H3. apply kv_aik_here.
   Case "leaf = a::leaf".
     intros.
     destruct p.
@@ -268,7 +269,7 @@ Proof.
     destruct neqk; symmetry in Heqneqk; [apply beq_nat_true_iff in Heqneqk|apply beq_nat_false_iff in Heqneqk].
     SCase "n = k".
       rewrite insert_leaf_cons_eq in H3.
-      inversion H3. apply aik_here. apply H. apply H0. 
+      inversion H3. apply kv_aik_here. apply H. apply H0. 
       rewrite Heqneqk. reflexivity.
       simpl. simpl in H2. omega.
     SCase "n <> k".
@@ -278,7 +279,7 @@ Proof.
        apply le_lt_or_eq_iff in Heqnlek. inversion Heqnlek.
        SSSCase "n < k".
          rewrite insert_leaf_cons_gt in H3.
-         inversion H3. apply aik_later.
+         inversion H3. apply kv_aik_later.
          apply insert_into_list_appears.
          apply H.
          apply H0.
@@ -288,21 +289,18 @@ Proof.
          apply ex_falso_quodlibet. apply Heqneqk. apply H4.
       SSCase "n > k".
         rewrite insert_leaf_cons_lt in H3.
-        inversion H3. apply aik_here.
+        inversion H3. apply kv_aik_here.
         apply H.
         apply H0.
         omega.
         simpl in H2. simpl. omega.
 Qed.
 
-
-
-
 Theorem insert_leaf_works : forall {X: Type} {b: nat} (k: nat) (v: X) (leaf left: list (nat * X)) (rightOption: option (list (nat * X))),
   b <> 0 -> kvl_sorted leaf -> not (appears_in_kvl k leaf) -> 
   length leaf <= mult b 2 ->
   insert_leaf b k v leaf = (left, rightOption) ->
-  appears_in_kvl k left \/ (exists right, rightOption = Some(right) /\ appears_in_kvl k right).
+  kv_appears_in_kvl k v left \/ (exists right, rightOption = Some(right) /\ kv_appears_in_kvl k v right).
 Proof.
   intros.
   remember (blt_nat (length leaf) (b * 2)) as blt_length_b.
@@ -381,80 +379,6 @@ Proof.
         inversion H3.
 Qed.
 
-
-
-Lemma insert_leaf_shaddow : forall (X: Type) (b: nat) (n: nat) (v x: X) (kvl: list (nat * X)),
-  b <> 0 -> length ((n,x) :: kvl) <= mult b 2 -> insert_leaf b n v ((n, x) :: kvl) = ((n, v) :: kvl, None).
-Proof.
-  intros.
-  
-  unfold insert_leaf. unfold insert_into_list.
-  rewrite ble_nat_symm. rewrite <- beq_nat_refl.
-  remember (ble_nat (length ((n,v) :: kvl)) (b * 2)) as lb2.
-  destruct lb2.
-  reflexivity.
-  symmetry in Heqlb2. apply ble_nat_false in Heqlb2.
-  unfold not in Heqlb2.
-  apply ex_falso_quodlibet.
-  apply Heqlb2. simpl in H0. simpl. apply H0.
-Qed.
-
-
-Lemma insert'_not_split_impl_space_left: forall {X: Type} (b: nat) k (v:X) kpl tree,
-  valid_bplustree b X (bptNode b X kpl) ->
-  ~ appears_in_tree k (bptNode b X kpl) ->
-  kvl_sorted kpl ->
-  insert' (height (bptNode b X kpl)) k v (bptNode b X kpl) = (tree, None) ->
-  length kpl < S (b*2).
-Proof.
-  intros.
-  
-  induction H1. 
-  Case "kvl_sorted_0".
-    simpl. omega.
-  Case "kvl_sorted_1".
-    simpl. destruct H. omega. omega.
-  Case "kvl_sorted_cons".
-    assert (length ((n1, x1) :: (n2, x2) :: lst) = S(length((n2, x2) :: lst))).
-      reflexivity.
-    rewrite H4. apply n_lt_m__Sn_lt_Sm. destruct b. destruct H. omega. omega.
-    admit.
-  
-    (*
-    set (insert' (height bptNode b X l) k v (bptNode b X ((n, b0) :: kpl))) as test.
-    intro.
-    hnf in test.
-    destruct kpl.
-      simpl. omega.
-      destruct p.
-      remember (ble_nat n k && blt_nat k n0).
-      destruct b2. hnf in test.
-      remember (insert' k v b0).
-      destruct p. destruct o. destruct p.
-      SCase "insert in child overflowed".
-        admit.
-      SCase "insert in child had room".
-        simpl in test. remember (ble_nat n n).  destruct b3.
-        remember (beq_nat n n). destruct b3.
-        
-        admit.
-        
-        
-        rewrite <- beq_nat_refl in Heqb0. inversion Heqb0.
-        rewrite ble_nat_symm in Heqb3. inversion Heqb3.
-        
-      
-        
-      destruct kpl.
-      admit.
-      
-  simpl.
-    admit.*)
-Admitted.
-
-
-
-
 Lemma insert_leaf_preserves_sort: forall (X: Type) b k (v:X) l l1 l2,
   kvl_sorted l ->
   insert_leaf b k v l = (l1, Some l2) ->
@@ -483,13 +407,13 @@ Proof.
   admit.
 Admitted.
 
-Lemma insert'_works_normal : forall (X: Type) (b k n: nat) (t1 t2: bplustree b X) (kpl: list (nat * bplustree b X)),
+Lemma insert'_works_normal : forall (X: Type) (b k n: nat) (v: X) (t1 t2: bplustree b X) (kpl: list (nat * bplustree b X)),
   valid_bplustree b X (bptNode b X kpl) ->
-  appears_in_tree k t2 ->
+  kv_appears_in_tree k v t2 ->
   find_subtree k kpl = Some (n, t1) ->
   ~ appears_in_tree k t1 ->
 
-  appears_in_tree k (bptNode b X (insert_into_list n t2 kpl)).
+  kv_appears_in_tree k v (bptNode b X (insert_into_list n t2 kpl)).
 Proof.
   intros. 
   remember (insert_into_list n t2 kpl) as kpl'.
@@ -509,7 +433,7 @@ Proof.
     rewrite Heqkpl'.
     inversion H.
     apply insert_preserves_sort; assumption.
-  apply appears_in_tree_when_appears_in_subtree_and_found with (kpl := kpl') (subtree := t2) (key := n); try reflexivity; try assumption. 
+  apply kv_appears_in_tree_when_appears_in_subtree_and_found with (kpl := kpl') (subtree := t2) (key := n); try reflexivity; try assumption. 
 Qed.
 
 Lemma insert'_leaf_disregards_counter: forall (X: Type) (b counter k: nat) (v: X) (kvl: list (nat * X)),
@@ -542,11 +466,11 @@ Theorem insert'_works : forall {X: Type} (counter b k: nat) (v: X) (kpl: list (n
   counter = (height (bptNode b X kpl)) ->
   insert' counter k v (bptNode b X kpl) = (left, rightOption) ->
   
-  (rightOption = None /\ appears_in_tree k left)
+  (rightOption = None /\ kv_appears_in_tree k v left)
     \/
   (exists split, exists right, rightOption = Some(split, right)
-      /\ ((k < split /\ appears_in_tree k left)
-			\/ (split <= k /\ appears_in_tree k right))).
+      /\ ((k < split /\ kv_appears_in_tree k v left)
+			\/ (split <= k /\ kv_appears_in_tree k v right))).
 Proof.
   induction counter.
   Case "counter = 0".
@@ -674,7 +598,7 @@ Proof.
           destruct p. inversion Heqp.
           inversion Heqp. clear Heqp.
           symmetry in Heqo.
-          assert (appears_in_tree k (bptLeaf b X l0)).
+          assert (kv_appears_in_tree k v (bptLeaf b X l0)).
             inversion Heqchild in H4. inversion H4.
             assert (length l < b*2).
               symmetry in Heqp0.
@@ -753,7 +677,7 @@ Proof.
                 inversion H.
                 omega.
               
-              apply appears_in_tree_when_appears_in_subtree_and_found with (kpl := kpl'') (subtree := b1) (key := n); try reflexivity; try assumption.
+              apply kv_appears_in_tree_when_appears_in_subtree_and_found with (kpl := kpl'') (subtree := b1) (key := n); try reflexivity; try assumption.
             SSSSSCase "appears in right subtree".
               symmetry in Heqo.
               assert (find_subtree k kpl = Some (n, child)) by assumption.
@@ -779,12 +703,12 @@ Proof.
                   assumption.
                 rewrite insert_into_list_last_twice in *; try assumption.
                 destruct witness1.
-                  apply ait_node_last; assumption.
+                  apply kv_ait_node_last; assumption.
                   destruct p.
                   rewrite <- app_comm_cons.
                   remember (witness1 ++ [(n, b1)]).
                   replace ((n1, b2) :: witness1 ++ [(n, b1), (witness, witness0)]) with ((n1, b2)::l0 ++ [(witness, witness0)]).
-                  apply appears_in_tree_when_appears_in_last_subtree; try assumption.
+                  apply kv_appears_in_tree_when_appears_in_last_subtree; try assumption.
                   rewrite Heql0.
                   rewrite <- app_assoc. simpl.
                   assumption.
@@ -827,7 +751,7 @@ Proof.
 				  apply H18 in H23.
 				  rewrite <- H21 in H23.
 				  assumption.
-				eapply appears_in_tree_when_appears_in_subtree_and_found.
+				eapply kv_appears_in_tree_when_appears_in_subtree_and_found.
 				  apply H22.
 				  apply H18.
 				  reflexivity.
@@ -852,146 +776,11 @@ Proof.
       do 2 destruct H. rewrite H in Heqo. inversion Heqo.
 Admitted.
 
-
-Theorem insert'_normal : forall {X: Type} {counter b: nat} (kpl: list (nat * bplustree b X)) (tree: bplustree b X) (k: nat) (v: X),
-  valid_bplustree b X (bptNode b X kpl) -> 
-  not (appears_in_tree k (bptNode b X kpl)) -> 
-  length kpl < S (mult b 2) ->
-  counter = (height (bptNode b X kpl)) ->
-  insert' counter k v (bptNode b X kpl) = (tree, None) -> 
-  
-  appears_in_tree k tree.
-Proof.
-  induction counter.
-  Case "counter = 0".
-    intros.
-    inversion H.
-    simpl in H2. 
-    destruct kpl. simpl in H6. exfalso. omega.
-    destruct p. inversion H2.
-  Case "counter = S counter". 
-    intros. 
-    simpl in H3.
-    remember (find_subtree k kpl).
-    destruct o.
-      destruct p.
-      remember (insert' counter k v b0) as insert_into_child.
-      destruct insert_into_child. destruct o.
-      SCase "child overflowed".
-        destruct p.
-        remember (ble_nat (length (insert_into_list n b1 (insert_into_list n0 b2 kpl))) (b * 2 + 1)) as fits_here.
-        destruct fits_here.
-        SSCase "the overflow fits on this level".
-          admit.
-        SSCase "the overflow doesn't fit here (bogus)".
-          (* needs to convince cut_list_right that it returns a list *)
-          admit.
-      SCase "child didn't overflow".
-        symmetry in Heqinsert_into_child.
-        symmetry in Heqo.
-        assert (n <= k).
-          (* needs proof based on Heqo *)
-          admit.
-        assert (find_subtree k kpl = Some (n, b0)) by assumption.
-        apply find_subtree_impl_kpl_app in Heqo.
-        destruct Heqo. destruct H6.
-        inversion H6.
-        assert (counter = height b0).
-          apply height_of_parent_one_bigger in H7. rewrite <- H7 in H2.
-          omega.
-          inversion H.
-          apply H15.
-        destruct b0.
-        SSCase "child was a leaf".
-          admit.
-        SSCase "child was a node".
-          inversion H.
-            clear H10. clear kpl0. clear H11. clear H12. clear H13. clear H14. clear H16. clear H17. clear H18.
-          rewrite H7 in H15.
-          apply all_values_single in H15.
-          apply valid_sub_bplustree_impl_valid_bplustree in H15.
-          
-          apply IHcounter in Heqinsert_into_child; try assumption.
-          inversion H3. rewrite H11. clear H3.
-          remember ((insert_into_list n b1 kpl)) as kpl'.
-          assert (length kpl = length kpl').
-            apply find_subtree_impl_key_appears in H5.
-            apply override_in_list_preserves_length with (k := n) (v := b1) in H5.
-            rewrite <- Heqkpl' in H5. apply H5.
-            inversion H. assumption.
-          assert (kvl_sorted kpl').
-            inversion H.
-            apply insert_preserves_sort with (k := n) (v := b1) in H19. 
-            rewrite Heqkpl'. assumption.
-          symmetry in Heqkpl'.
-          assert (insert_into_list n b1 kpl = kpl') by assumption.
-          apply insert_into_list_app in Heqkpl'.
-          destruct Heqkpl'. destruct H13.
-          rewrite H13 in H11.
-          rewrite <- H11.
-          destruct witness2.
-          SSSCase "found subtree was the last subtree".
-            destruct witness1. simpl in H13. rewrite H13 in H3. simpl in H3.
-            inversion H. rewrite H3 in H18. exfalso. omega.
-            rewrite <- app_comm_cons in H11. destruct p.
-            rewrite H13 in H10.
-            apply appears_in_tree_when_appears_in_last_subtree; try assumption.
-          SSSCase "found subtree was not the last".
-            destruct p.
-
-            assert (kvl_sorted (witness1 ++ (n, b1) :: (n0, b0) :: witness2)).
-              rewrite H13 in H10. apply H10.
-            assert (kvl_sorted (witness ++ (n, b1) :: witness0)).
-              rewrite H7 in H12.
-              rewrite override_in_list_app in H12.
-              rewrite <- H12 in H10. apply H10. 
-              inversion H. 
-              rewrite H7 in H23.
-              apply H23.
-            assert (witness0 = (n0, b0)::witness2). 
-              rewrite H7 in H12.
-              rewrite override_in_list_app in H12.
-              
-              rewrite H13 in H12.
-              apply kvl_sorted_elim_common_head in H12.
-              apply H12.
-              apply H16.
-              apply H14.
-              inversion H. 
-              rewrite H7 in H24.
-              apply H24.
-            clear H16.
-
-            assert (k < n0).
-              destruct H8. rewrite H8 in H17.
-              inversion H17.
-              do 3 destruct H8.
-              inversion H8.
-              rewrite H16 in H17.
-              inversion H17.
-              subst.
-              omega.
-            apply appears_in_tree_when_appears_in_subtree; try assumption.
-              omega.
-              
-          unfold not. unfold not in H0. intro. apply H0.
-          rewrite H7.
-          
-          admit.
-          admit.
-
-
-
-    inversion H.
-    apply find_subtree_finds_a_subtree with (sk := k) in H.
-    do 2 destruct H. rewrite H in Heqo. inversion Heqo.
-Admitted.
-
 Theorem insert_works : forall {X: Type} {b: nat} (t t1: bplustree b X) (k: nat) (v: X),
   valid_bplustree b X t -> 
   ~appears_in_tree k t -> 
   insert k v t = t1 -> 
-  appears_in_tree k t1.
+  kv_appears_in_tree k v t1.
 Proof.
   intros.
   induction H.
@@ -1007,17 +796,17 @@ Proof.
 	    
 	  symmetry in Heqil. assert (insert_leaf b k v kvl = (l, Some ((n,x)::l0))) by assumption.
 	  apply insert_leaf_works in Heqil; try assumption.
-	    rewrite <- H1. apply appears_in_split_node_appears_in_lists. destruct Heqil. 
+	    rewrite <- H1. apply kv_appears_in_split_node_appears_in_lists. destruct Heqil. 
 	    apply insert_leaf_preserves_sort in H5; assumption; assumption.
 	    apply insert_leaf_preserves_sort in H5; assumption; assumption.
 	    simpl. reflexivity.
 	    destruct Heqil. left. assumption.
-	    inversion H6. right. do 3 destruct H6. inversion H7. inversion H6. rewrite H11. assumption.
+	    inversion H6. right. destruct H6. inversion H7. inversion H8. rewrite H11. assumption.
 	    unfold not. intro. apply H0. apply ait_leaf. apply H6.
 	    assumption.
 	SCase "insert_normal".
 	  symmetry in Heqil. apply insert_leaf_normal in Heqil; try assumption. rewrite <- H1. 
-	  apply ait_leaf; try assumption. unfold not. intro. unfold not in H0.
+	  apply kv_ait_leaf; try assumption. unfold not. intro. unfold not in H0.
 	  eapply appears_kvl_appears_leaf_tree in H4. apply H0. apply H4. 
 	  apply insert_leaf_not_split_impl_space_left in Heqil. assumption.
 	  unfold not. unfold not in H0. intros. apply H0. apply ait_leaf. assumption.
@@ -1034,10 +823,10 @@ Proof.
       inversion Heqp. destruct H9.  inversion H9. do 3 destruct H9.
       inversion H9. subst. destruct H10.
       SSCase "appears in left".
-        apply ait_node_here. destruct H1. assumption. omega.
+        apply kv_ait_node_here. destruct H1. assumption. omega.
       SSCase "appears in right".
 		destruct H1.
-		apply ait_node_last. assumption. omega.
+		apply kv_ait_node_last. assumption. omega.
     SCase "node didn't overflow".
       inversion Heqp. 
       SSCase "appears in left".
