code/KvAppearsInTree.v
@@ -5,56 +5,56 @@ Require Export ValidBPlusTree.
 Require Export SortingProofs.
 Require Export FindSubtreeProofs.
 
-Lemma appears_in_split_node_appears_in_lists: forall {X: Type} b k n left right, 
+Lemma kv_appears_in_split_node_appears_in_lists: forall {X: Type} b k v n left right, 
   kvl_sorted (left ++ right) ->
   key_at_index 0 right = Some n ->
-  appears_in_kvl k left \/ appears_in_kvl k right ->
-  appears_in_tree k (bptNode b X [(0, bptLeaf b X left), (n, bptLeaf b X right)]).
+  kv_appears_in_kvl k v left \/ kv_appears_in_kvl k v right ->
+  kv_appears_in_tree k v (bptNode b X [(0, bptLeaf b X left), (n, bptLeaf b X right)]).
 Proof.
   intros. destruct H1. 
   Case "Left hand side".
-    apply ait_node_here. apply ait_leaf. assumption. destruct right.
+    apply kv_ait_node_here. apply kv_ait_leaf. assumption. destruct right.
     simpl in H0. inversion H0. inversion H0. destruct p. inversion H3. subst.
-    apply appears_in_kvl_app in H1. do 3 destruct H1. subst. 
+    apply kv_appears_in_kvl_app in H1. do 2 destruct H1. subst. 
     rewrite <- app_assoc in H. apply kvl_sorted_app with (l1:=witness) in H. destruct H.
     apply kvl_sorted_key_across_app in H1. omega.
   Case "Right hand side".
-    apply ait_node_last. apply ait_leaf. assumption. 
+    apply kv_ait_node_last. apply kv_ait_leaf. assumption. 
     SCase "n <=".
       inversion H0. destruct right. inversion H3. destruct p. inversion H3. subst. remember (beq_nat n k).
       destruct b0. symmetry in Heqb0. apply beq_nat_true in Heqb0. subst. omega.
-      apply appears_cons in H1. apply appears_in_kvl_app in H1. do 3 destruct H1. subst.
+      apply kv_appears_cons in H1. apply kv_appears_in_kvl_app in H1. do 2 destruct H1. subst.
       apply kvl_sorted_app with (l1:=left) in H. inversion H. 
       apply kvl_sorted_key_across_app in H2.  omega. symmetry in Heqb0. 
       apply beq_nat_false in Heqb0. omega.
 Qed.
 
-Lemma appears_in_tree_when_appears_in_subtree: forall (X: Type) (b k k1 k2: nat) (t1 t2: bplustree b X) (l1 l2: list (nat * bplustree b X)),
-  appears_in_tree k t1 -> 
+Lemma kv_appears_in_tree_when_appears_in_subtree: forall (X: Type) (b k k1 k2: nat) (v: X) (t1 t2: bplustree b X) (l1 l2: list (nat * bplustree b X)),
+  kv_appears_in_tree k v t1 -> 
   k1 <= k < k2 ->
   kvl_sorted (l1 ++ (k1, t1) :: (k2, t2)::l2) ->
-  appears_in_tree k (bptNode b X (l1 ++ (k1, t1) :: (k2, t2)::l2)).
+  kv_appears_in_tree k v (bptNode b X (l1 ++ (k1, t1) :: (k2, t2)::l2)).
 Proof.
   intros.
   induction l1.
   Case "l1 = []".
     simpl.
-   apply ait_node_here; assumption.
+   apply kv_ait_node_here; assumption.
      destruct a. rewrite <- app_comm_cons.
      destruct l1. 
        simpl.
-       apply ait_node_later. apply IHl1. 
+       apply kv_ait_node_later. apply IHl1. 
          simpl. simpl in H1. apply list_tail_is_sorted in H1. apply H1.
          omega.
        rewrite <- app_comm_cons. destruct p.
        destruct l1.
-         simpl. apply ait_node_later. simpl in IHl1. apply IHl1. 
+         simpl. apply kv_ait_node_later. simpl in IHl1. apply IHl1. 
            simpl in H1. apply list_tail_is_sorted in H1. apply H1.
            simpl in H1. inversion H1. inversion H4.
            apply blt_nat_true in H15. omega.
            
          rewrite <- app_comm_cons. destruct p.
-         apply ait_node_later. apply IHl1.
+         apply kv_ait_node_later. apply IHl1.
            apply list_tail_is_sorted in H1. apply H1.
            simpl in H1.
            inversion H1.
@@ -62,29 +62,29 @@ Proof.
            omega.
 Qed.
 
-Lemma appears_in_tree_when_appears_in_last_subtree: forall (X: Type) (b k k1 k2: nat) (t1 t2: bplustree b X) (l1: list (nat * bplustree b X)),
-  appears_in_tree k t1 -> 
+Lemma kv_appears_in_tree_when_appears_in_last_subtree: forall (X: Type) (b k k1 k2: nat) (v: X) (t1 t2: bplustree b X) (l1: list (nat * bplustree b X)),
+  kv_appears_in_tree k v t1 -> 
   k1 <= k ->
   kvl_sorted ((k2,t2)::l1 ++ [(k1, t1)]) ->
-  appears_in_tree k (bptNode b X ((k2,t2)::l1 ++ [(k1, t1)])).
+  kv_appears_in_tree k v (bptNode b X ((k2,t2)::l1 ++ [(k1, t1)])).
 Proof.
   intros. generalize dependent k2. generalize dependent t2.
   induction l1.
   Case "l1 = []".
     intros.
     simpl.
-    apply ait_node_last; assumption.
+    apply kv_ait_node_last; assumption.
   Case "l1 = a::l1". destruct a.
     intros.
     destruct l1.
       simpl.
-      apply ait_node_later. apply ait_node_last; assumption.
+      apply kv_ait_node_later. apply kv_ait_node_last; assumption.
       simpl in H1.
       inversion H1. inversion H4.
       apply blt_nat_true in H15. omega.
       destruct p.
       repeat rewrite <- app_comm_cons.
-      apply ait_node_later.
+      apply kv_ait_node_later.
       apply IHl1.
       simpl in H1. simpl. apply list_tail_is_sorted in H1. apply H1.
       
@@ -93,32 +93,32 @@ Proof.
       omega.
 Qed.    
 
-Lemma appears_in_known_subtree: forall {X:Type} b n1 k n2 t1 t2 kpl kpl', 
+Lemma kv_appears_in_known_subtree: forall {X:Type} b n1 k v n2 t1 t2 kpl kpl', 
   kpl = bptNode b X ((n1, t1) :: (n2, t2) :: kpl') ->
   n1 <= k < n2 ->
-  appears_in_tree k (kpl) ->
-  appears_in_tree k t1.
+  kv_appears_in_tree k v kpl ->
+  kv_appears_in_tree k v t1.
 Proof.
   intros. induction H1; inversion H; subst; try (exfalso; omega).
   Case "ait_here".
     assumption.
 Qed.
 
-Lemma appears_in_later_subtree: forall {X:Type} b n1 k n2 n3 t1 t2 t3 kpl kpl', 
+Lemma kv_appears_in_later_subtree: forall {X:Type} b n1 k v n2 n3 t1 t2 t3 kpl kpl', 
   kpl = bptNode b X ((n1, t1) :: (n2, t2) :: (n3, t3) :: kpl') ->
   kvl_sorted ((n1, t1) :: (n2, t2) :: (n3, t3) :: kpl') ->
   k >= n2 ->
-  appears_in_tree k kpl ->
-  appears_in_tree k (bptNode b X ((n2, t2) :: (n3, t3) :: kpl')).
+  kv_appears_in_tree k v kpl ->
+  kv_appears_in_tree k v (bptNode b X ((n2, t2) :: (n3, t3) :: kpl')).
 Proof. 
   intros. induction H2; inversion H; subst; try (exfalso; omega).
   assumption.
 Qed.
 
-Lemma appears_in_tree_before_kpl_start_false: forall {X:Type} b n k t kpl, 
+Lemma kv_appears_in_tree_before_kpl_start_false: forall {X:Type} b n k v t kpl, 
   n > k ->
   kvl_sorted ((n, t) :: kpl) ->
-  appears_in_tree k (bptNode b X ((n, t) :: kpl)) ->
+  kv_appears_in_tree k v (bptNode b X ((n, t) :: kpl)) ->
   False.
 Proof.
   intros. remember (bptNode b X ((n, t) :: kpl)). destruct H1; inversion Heqb0; subst.
@@ -127,10 +127,10 @@ Proof.
   omega.
 Qed.
 
-Lemma appears_in_tree_two_last: forall {X: Type} b n1 n2 t1 t2 k,
+Lemma kv_appears_in_tree_two_last: forall {X: Type} b n1 n2 t1 t2 k v,
   k >= n2 ->
-  appears_in_tree k (bptNode b X [(n1, t1), (n2, t2)]) ->
-  appears_in_tree k t2.
+  kv_appears_in_tree k v (bptNode b X [(n1, t1), (n2, t2)]) ->
+  kv_appears_in_tree k v t2.
 Proof. 
   intros. remember (bptNode b X [(n1, t1), (n2, t2)]). destruct H0. inversion Heqb0.
   inversion Heqb0. subst. assumption. inversion Heqb0. subst. exfalso. omega.
@@ -144,15 +144,15 @@ Qed.
 (* Informal: We know k appears in the parent tree, and we know that find_subtree
  * returns the subtree when searching for k, so hence k must also appear in the
  * subtree *)
-Lemma appears_in_subtree_when_appears_in_tree_and_found: 
-    forall (X: Type) (b k key: nat) 
+Lemma kv_appears_in_subtree_when_appears_in_tree_and_found: 
+    forall (X: Type) (b k key: nat) (v: X)
     (subtree: bplustree b X) (kpl: list (nat * bplustree b X)),
   
-  kvl_sorted(kpl) ->
-  appears_in_tree k (bptNode b X kpl) ->
+  kvl_sorted kpl ->
+  kv_appears_in_tree k v (bptNode b X kpl) ->
   find_subtree k kpl = Some (key, subtree) ->
   
-  appears_in_tree k subtree.
+  kv_appears_in_tree k v subtree.
 Proof.
   intros. induction kpl. 
   Case "kpl = []".
@@ -163,23 +163,23 @@ Proof.
   	    destruct p. remember (ble_nat n k && blt_nat k n0) as loc. destruct loc. 
   	      unfold find_subtree in H1. rewrite <- Heqloc in H1. inversion H1. 
 	      symmetry in Heqloc. unfold andb in Heqloc. 
-	      apply ble_and_blt_true in Heqloc. eapply appears_in_known_subtree in H0. 
+	      apply ble_and_blt_true in Heqloc. eapply kv_appears_in_known_subtree in H0. 
 	      apply H0. rewrite H4. reflexivity. assumption. 
 	  symmetry in Heqloc. apply ble_and_blt_false in Heqloc.
 	  destruct kpl.
 	  SCase "kpl = []".
 	    destruct Heqloc.
-	    apply appears_in_tree_before_kpl_start_false in H0. inversion H0.
+	    apply kv_appears_in_tree_before_kpl_start_false in H0. inversion H0.
 	    assumption. assumption.
-	    apply appears_in_tree_two_last in H0.  apply find_subtree_later in H1. 
-	    apply find_subtree_one_impl_found in H1. destruct H1. rewrite <- H3. assumption. 
+	    apply kv_appears_in_tree_two_last in H0.  apply find_subtree_later in H1. 
+	    apply find_subtree_one_impl_found in H1. destruct H1. rewrite <- H3. assumption.  
 	    right. assumption. right. assumption. assumption. assumption.
 	  SCase "kpl = p :: kpl".
 	    destruct p.	    
 	    apply IHkpl. apply list_tail_is_sorted in H. assumption. 
 	    destruct Heqloc.
-	      apply appears_in_tree_before_kpl_start_false in H0; try assumption. inversion H0.
-	      eapply appears_in_later_subtree in H0. apply H0. reflexivity.  assumption. assumption.
+	      apply kv_appears_in_tree_before_kpl_start_false in H0; try assumption. inversion H0.
+	      eapply kv_appears_in_later_subtree in H0. apply H0. reflexivity.  assumption. assumption.
 	    eapply find_subtree_later in Heqloc. apply Heqloc. apply H. apply H1.
 Qed.
   
@@ -187,19 +187,20 @@ Qed.
    * when appears_in_tree k parent tries to identify the subtree, it will find
    * the same as find_subtree, and because it exists in the subtree, it must also
    * exists in the parent tree *)
-Lemma appears_in_tree_when_appears_in_subtree_and_found: forall (X: Type) (b k key: nat) (parent subtree: bplustree b X) (kpl: list (nat * bplustree b X)),
+Lemma kv_appears_in_tree_when_appears_in_subtree_and_found: forall (X: Type) (b k key: nat) (v: X) (parent subtree: bplustree b X) (kpl: list (nat * bplustree b X)),
   2 <= length kpl ->
   kvl_sorted kpl ->
   parent = bptNode b X kpl ->
   find_subtree k kpl = Some (key, subtree) ->
-  appears_in_tree k subtree ->
+  kv_appears_in_tree k v subtree ->
 
-  appears_in_tree k parent.
+  kv_appears_in_tree k v parent.
 Proof.
   intros.
   rewrite H1.
   assert (key <= k).
-    apply find_subtree_returns_a_lesser_key in H2; try assumption. omega.
+    apply find_subtree_returns_a_lesser_key in H2; try assumption.
+    omega.
   apply find_subtree_impl_kpl_app in H2.
   do 2 destruct H2.
   inversion H2. clear H2.
@@ -213,29 +214,14 @@ Proof.
       rewrite <- app_comm_cons in H5.
       rewrite H5.
       rewrite H5 in H0.
-      apply appears_in_tree_when_appears_in_last_subtree; assumption.
+      apply kv_appears_in_tree_when_appears_in_last_subtree; assumption.
   Case "witness = p::witness".
     destruct p.
     inversion H6. inversion H2.
     do 3 destruct H2.
     inversion H2. clear H2. inversion H7. subst.
-    apply appears_in_tree_when_appears_in_subtree; try assumption.
+    apply kv_appears_in_tree_when_appears_in_subtree; try assumption.
       omega.
-Qed.
-
-Lemma not_appears_in_subtree_when_not_appears_in_tree_and_found : forall (X: Type) (b k key: nat) (child: bplustree b X) (kpl: list (nat * bplustree b X)),
-  valid_bplustree b X (bptNode b X kpl) ->
-  ~appears_in_tree k (bptNode b X kpl) ->
-  find_subtree k kpl = Some(key, child) ->
-  ~appears_in_tree k child.
-Proof.
-  intros.
-  inversion H.
-  unfold not.
-  intro.
-  apply H0.
-  apply appears_in_tree_when_appears_in_subtree_and_found with (key := key) (subtree := child) (kpl := kpl);
-            try assumption; try reflexivity.
 Qed.
 
 (*
